examples/unit-tests/NegativeTests.False.fst
@@ -1,6 +1,0 @@
-module NegativeTests.False (* #284 *)
-val foo : f:(unit -> Tot bool){f () = true}
-          -> Tot (r:bool {r = f () /\ r = true})
-let foo f = f ()
-val bar : unit -> Pure bool (requires True) (ensures (fun _ -> False))
-let bar () = foo (fun x -> false)
