examples/unit-tests/NegativeTests.ShortCircuiting.fst
@@ -1,8 +1,0 @@
-module NegativeTests.ShortCircuiting
-
-type Bad : bool -> Type
-val bad : x:int -> Tot (b:bool{Bad b})
-let rec bad x = true || bad (x-1)
-
-val ff : unit -> Lemma (ensures False)
-let ff u = ignore (false && (0 = 1))
